Working on conversion between [System] and [PSystem]

src/PredMsgFacts.v
@@ -16,13 +16,41 @@ Definition pToSystem (psys: PSystem): System :=
      sys_inits := psys_inits psys;
      sys_rules := map pToRule (psys_rules psys) |}.
 
+Definition pToTMsg (ts: TrsId) (rqin: Msg) (pmsg: PMsgSig): TMsg :=
+  {| tmsg_msg := {| msg_id := pmsg_mid (projT2 pmsg);
+                    msg_value := pmsg_val (projT2 pmsg)
+                 |};
+     tmsg_info := Some {| tinfo_tid := ts; tinfo_rqin := rqin :: nil |}
+  |}.
+
+Definition pToTState (ts: TrsId) (rqin: Msg) (pst: PState): TState :=
+  {| tst_oss := pst_oss pst;
+     tst_msgs := map (pToTMsg ts rqin) (pst_msgs pst);
+     tst_tid := ts |}.
+
+Definition pToTLabel (ts: TrsId) (rqin: Msg) (plbl: PLabel): TLabel :=
+  match plbl with
+  | PlblIn min => RlblIn (pToTMsg ts rqin (existT _ _ min))
+  | PlblOuts oprule mins mouts =>
+    RlblOuts (lift pToRule oprule)
+             (map (pToTMsg ts rqin) mins)
+             (map (pToTMsg ts rqin) mouts)
+  end.
+
+Definition pToTHistory (ts: TrsId) (rqin: Msg) (phst: PHistory): THistory :=
+  map (pToTLabel ts rqin) phst.
+
 Theorem steps_pred_ok:
   forall sys st1 thst st2 ts rqin mouts,
     steps_det sys st1 thst st2 ->
     Atomic sys ts rqin thst mouts ->
-    forall psys pst1 phst pst2,
+    forall psys,
       pToSystem psys = sys ->
-      steps_pred psys pst1 phst pst2.
+      exists pst1 phst pst2,
+        pToTState ts rqin pst1 = st1 /\
+        pToTState ts rqin pst2 = st2 /\
+        behaviorOf psys phst = behaviorOf sys thst /\
+        steps_pred psys pst1 phst pst2.
 Proof.
 Admitted.
 
